src/coq/Util.v
@@ -892,3 +892,126 @@ Fixpoint find_map {A B} (f : A -> option B) (l : list A) : option B :=
             end
   end.
 
+
+Definition opt_compose {A B C} (g:B -> C) (f:A -> option B) : A -> option C :=
+  fun a => option_map g (f a).
+
+Fixpoint option_iter {A} (f:A -> option A) (a:A) (n:nat) : option A :=
+  match n with
+  | 0 => Some a
+  | S n' => match f a with
+            | Some a' => option_iter f a' n'
+            | None => None
+            end
+  end.
+
+Arguments option_map {_ _} _ _.
+
+Lemma option_map_id : forall A (a : option A), option_map id a = a.
+Proof.
+  unfold option_map; destruct a; auto.
+Qed.
+
+Lemma option_map_ext : forall A B (f g:A->B),
+  (forall a, f a = g a) ->
+  forall oa, option_map f oa = option_map g oa.
+Proof.
+  intros. destruct oa. simpl. rewrite H; auto. auto.
+Qed.
+
+Lemma option_map_some_inv {A B} : forall (o:option A) (f : A -> B) (b:B),
+  option_map f o = Some b ->
+  exists a, o = Some a /\ f a = b.
+Proof.
+  destruct o; simpl; intros; inversion H; eauto.
+Qed.
+
+Definition option_prop {A} (P: A -> Prop) (a:option A) :=
+  match a with
+    | None => True
+    | Some a' => P a'
+  end.
+
+Definition option_bind {A B} (m:option A) (f:A -> option B) : option B :=
+  match m with
+  | Some a => f a
+  | None => None
+  end.
+
+Definition option_bind2 {A B C} (m: option (A * B)) (f: A -> B -> option C) : option C :=
+  match m with
+  | Some (a, b) => f a b
+  | None => None
+  end.
+
+Module OptionNotations.
+
+  Notation "'do' x <- m ; f" := (option_bind m (fun x => f)) 
+    (at level 200, x ident, m at level 100, f at level 200).
+
+  Notation "'do' x , y <- m ; f" := (option_bind2 m (fun x y => f))
+    (at level 200, x ident, y ident, m at level 100, f at level 200).
+
+End OptionNotations.
+
+Tactic Notation "not_var" constr(t) :=
+  try (is_var t; fail 1 "not_var").
+
+Create HintDb inversions.
+Tactic Notation "iauto" := auto 10 with inversions.
+Tactic Notation "ieauto" := eauto 10 with inversions.
+
+Definition map_prod {A B C D} (p:A * B) (f:A -> C) (g:B -> D) : (C * D) :=
+  (f (fst p), g (snd p)).
+
+Definition flip := @Basics.flip.
+Definition comp := @Basics.compose.
+
+Notation "g `o` f" := (Basics.compose g f) 
+  (at level 40, left associativity).
+
+Lemma map_prod_distr_comp : forall A B C D E F
+  (p:A * B) (f1:A -> C) (f2:B -> D) (g1:C -> E) (g2:D -> F),
+  map_prod (map_prod p f1 f2) g1 g2 =
+  map_prod p (g1 `o` f1) (g2 `o` f2).
+Proof.
+  unfold map_prod, Basics.compose. auto.
+Qed.
+
+Definition map_snd {A B C} (f:B -> C) : list (A * B) -> list (A * C) :=
+  map (fun ab : A * B => let (a, b) := ab in (a, f b)).
+
+Import OptionNotations.
+
+Lemma option_bind_assoc {A B C} : forall (o:option A) (p:A -> option B) (q:B -> option C),
+   (do y <- (do x <- o; p x); q y) = (do x <- o; do y <- p x; q y).
+Proof.
+  intros. destruct o; auto.
+Qed.
+
+Lemma option_bind_some_inv {A B} : forall (o:option A) (p:A -> option B) (b:B),
+  (do x <- o; p x) = Some b ->
+  exists a, o = Some a /\ p a = Some b.
+Proof.
+  intros. destruct o. eexists. eauto. inversion H.
+Qed.
+
+Lemma option_bind_None : forall A B (m : option A),
+  (do x <- m; (None(A := B))) = None.
+Proof.
+  destruct m; auto.
+Qed.
+
+Lemma option_bind_some : forall A (m : option A),
+  (do x <- m; Some x) = m.
+Proof.
+  destruct m; auto.
+Qed.
+
+Tactic Notation "inv_bind" hyp(H) :=
+  repeat rewrite option_bind_assoc in H;
+    match type of H with
+    | option_bind ?o ?p = Some ?b => 
+      let hy := fresh H in
+      destruct o eqn:hy; [|discriminate]; simpl in H
+    end.
